code/ecdsa/Hacl.Impl.EC.Masking.ScalarAccess.fst
@@ -1,0 +1,83 @@
+module Hacl.Impl.EC.Masking.ScalarAccess
+
+
+open FStar.HyperStack.All
+open FStar.HyperStack
+module ST = FStar.HyperStack.ST
+
+open Lib.IntTypes
+open Lib.Buffer
+open Lib.Loops
+
+open Spec.ECC
+open Spec.ECC.Curves
+open Hacl.Impl.EC.Masking
+
+#set-options " --z3rlimit 200"
+
+
+inline_for_extraction noextract
+val getScalarBit_leftEndian: #c: curve 
+  -> #buf_type: buftype 
+  -> s:lbuffer_t buf_type uint8 (getScalarLenBytes c) 
+  -> n:size_t{v n < v (getScalarLen c)}
+  -> Stack uint64
+    (requires fun h0 -> live h0 s)
+    (ensures  fun h0 r h1 -> h0 == h1 /\ r == ith_bit #c (as_seq h0 s) (v n) /\ v r <= 1)
+
+let getScalarBit_leftEndian #c #buf_type s n =
+  let h0 = ST.get () in
+  assert_norm (1 = pow2 1 - 1);
+  assert (v (mod_mask #U8 #SEC 1ul) == v (u8 1)); 
+  to_u64 ((s.(getScalarLenBytes c -. 1ul -. n /. 8ul) >>. (n %. 8ul)) &. u8 1)
+
+
+inline_for_extraction noextract
+val getScalarBit_l: #c: curve 
+  -> #buf_type: buftype 
+  -> s:lbuffer_t buf_type uint8 (getScalarLenBytes c) 
+  -> n:size_t{v n < v (getScalarLen c)}
+  -> Stack uint64
+    (requires fun h0 -> live h0 s)
+    (ensures  fun h0 r h1 -> h0 == h1 /\ r == ith_bit #c (as_seq h0 s) (v n) /\ v r <= 1)
+
+let getScalarBit_l #c #b s n = 
+  push_frame();
+    let h0 = ST.get() in 
+    let temp = create (size 1) (u64 0) in 
+    let inv h i = modifies (loc temp) h0 h /\ live h temp in 
+    for 0ul (getScalarLen c) inv (fun i -> 
+      let bit = getScalarBit_leftEndian s n in 
+      assert(bit == ith_bit (as_seq h0 s) (v n));
+      
+      let mask = neq_mask (size_to_uint64 n) (size_to_uint64 i) in 
+	neq_mask_lemma (size_to_uint64 n) (size_to_uint64 i);
+      copy_conditional_u64 bit temp mask);
+  let result = index temp (size 0) in
+  admit();
+  pop_frame();
+  result
+    
+
+[@ CInline]
+inline_for_extraction noextract  
+val getScalar_4: #buf_type: buftype 
+  -> scalar: lbuffer_t buf_type uint8 (size 32) -> i: size_t {v i < 64} -> 
+  Stack uint32 
+    (requires fun h -> live h scalar)
+    (ensures fun h0 _ h1 -> True)
+
+let getScalar_4 #a scalar i = 
+  let half = shift_right i 1ul in 
+    shift_right_lemma i 1ul;
+  let word = to_u32 (index scalar half) in 
+  let bitShift : size_t = logand i (size 1) in 
+    logand_mask i (size 1) 1; 
+  let bitShiftAsPrivate = size_to_uint32 bitShift in 
+  let mask : uint32 = cmovznz01 (u32 0xf0) (u32 0x0f) bitShiftAsPrivate in  
+  let shiftMask = cmovznz01 (size 0x4) (size 0x0) bitShift in
+  let result : uint32 = logand word mask in 
+  let result : uint32 = shift_right result shiftMask in 
+  result
+
+
